updated constructor removal edits to keep Type/Coercion/Cast, only remove Tick

examples/ghc/lib/Core.v
@@ -491,7 +491,9 @@ with DataConRep : Type
   (dcr_stricts : list StrictnessMark) (dcr_bangs : list HsImplBang)
    : DataConRep
 with Var : Type
-  := | Mk_Id (varName : Name.Name) (realUnique : BinNums.N) (varType : Type_)
+  := | Mk_TyVar (varName : Name.Name) (realUnique : BinNums.N) (varType : Kind)
+   : Var
+  |  Mk_Id (varName : Name.Name) (realUnique : BinNums.N) (varType : Type_)
   (idScope : IdScope) (id_details : IdDetails) (id_info : IdInfo)
    : Var
 with IdDetails : Type
@@ -504,6 +506,7 @@ with IdDetails : Type
   |  FCallId : unit -> IdDetails
   |  TickBoxOpId : TickBoxOp -> IdDetails
   |  Mk_DFunId : bool -> IdDetails
+  |  CoVarId : IdDetails
   |  Mk_JoinId : BasicTypes.JoinArity -> IdDetails
 with RecSelParent : Type
   := | RecSelData : TyCon -> RecSelParent
@@ -662,6 +665,9 @@ Inductive Expr b : Type
    : (Expr b) ->
      b ->
      Type_ -> list ((fun b_ => (AltCon * list b_ * Expr b_)%type%type) b) -> Expr b
+  |  Cast : (Expr b) -> Coercion -> Expr b
+  |  Mk_Type : Type_ -> Expr b
+  |  Mk_Coercion : Coercion -> Expr b
 with Bind b : Type
   := | NonRec : b -> (Expr b) -> Bind b
   |  Rec : list (b * (Expr b))%type -> Bind b.
@@ -756,6 +762,12 @@ Inductive AnnExpr' bndr annot : Type
    : (AnnBind bndr annot) ->
      ((fun bndr_ annot_ => (annot_ * AnnExpr' bndr_ annot_)%type%type) bndr annot) ->
      AnnExpr' bndr annot
+  |  AnnCast
+   : ((fun bndr_ annot_ => (annot_ * AnnExpr' bndr_ annot_)%type%type) bndr
+      annot) ->
+     (annot * Coercion)%type -> AnnExpr' bndr annot
+  |  AnnType : Type_ -> AnnExpr' bndr annot
+  |  AnnCoercion : Coercion -> AnnExpr' bndr annot
 with AnnBind bndr annot : Type
   := | AnnNonRec
    : bndr ->
@@ -866,6 +878,12 @@ Arguments Let {_} _ _.
 
 Arguments Case {_} _ _ _ _.
 
+Arguments Cast {_} _ _.
+
+Arguments Mk_Type {_} _.
+
+Arguments Mk_Coercion {_} _.
+
 Arguments NonRec {_} _ _.
 
 Arguments Rec {_} _.
@@ -881,6 +899,12 @@ Arguments AnnApp {_} {_} _ _.
 Arguments AnnCase {_} {_} _ _ _ _.
 
 Arguments AnnLet {_} {_} _ _.
+
+Arguments AnnCast {_} {_} _ _.
+
+Arguments AnnType {_} {_} _.
+
+Arguments AnnCoercion {_} {_} _.
 
 Arguments AnnNonRec {_} {_} _ _.
 
@@ -2036,24 +2060,38 @@ Definition dcr_stricts (arg_0__ : DataConRep) :=
   end.
 
 Definition idScope (arg_0__ : Var) :=
-  let 'Mk_Id _ _ _ idScope _ _ := arg_0__ in
-  idScope.
+  match arg_0__ with
+  | Mk_TyVar _ _ _ =>
+      GHC.Err.error (GHC.Base.hs_string__
+                     "Partial record selector: field `idScope' has no match in constructor `Mk_TyVar' of type `Var'")
+  | Mk_Id _ _ _ idScope _ _ => idScope
+  end.
 
 Definition id_details (arg_0__ : Var) :=
-  let 'Mk_Id _ _ _ _ id_details _ := arg_0__ in
-  id_details.
+  match arg_0__ with
+  | Mk_TyVar _ _ _ =>
+      GHC.Err.error (GHC.Base.hs_string__
+                     "Partial record selector: field `id_details' has no match in constructor `Mk_TyVar' of type `Var'")
+  | Mk_Id _ _ _ _ id_details _ => id_details
+  end.
 
 Definition realUnique (arg_0__ : Var) :=
-  let 'Mk_Id _ realUnique _ _ _ _ := arg_0__ in
-  realUnique.
+  match arg_0__ with
+  | Mk_TyVar _ realUnique _ => realUnique
+  | Mk_Id _ realUnique _ _ _ _ => realUnique
+  end.
 
 Definition varName (arg_0__ : Var) :=
-  let 'Mk_Id varName _ _ _ _ _ := arg_0__ in
-  varName.
+  match arg_0__ with
+  | Mk_TyVar varName _ _ => varName
+  | Mk_Id varName _ _ _ _ _ => varName
+  end.
 
 Definition varType (arg_0__ : Var) :=
-  let 'Mk_Id _ _ varType _ _ _ := arg_0__ in
-  varType.
+  match arg_0__ with
+  | Mk_TyVar _ _ varType => varType
+  | Mk_Id _ _ varType _ _ _ => varType
+  end.
 
 Definition sel_naughty (arg_0__ : IdDetails) :=
   match arg_0__ with
@@ -2082,6 +2120,9 @@ Definition sel_naughty (arg_0__ : IdDetails) :=
   | Mk_DFunId _ =>
       GHC.Err.error (GHC.Base.hs_string__
                      "Partial record selector: field `sel_naughty' has no match in constructor `Mk_DFunId' of type `IdDetails'")
+  | CoVarId =>
+      GHC.Err.error (GHC.Base.hs_string__
+                     "Partial record selector: field `sel_naughty' has no match in constructor `CoVarId' of type `IdDetails'")
   | Mk_JoinId _ =>
       GHC.Err.error (GHC.Base.hs_string__
                      "Partial record selector: field `sel_naughty' has no match in constructor `Mk_JoinId' of type `IdDetails'")
@@ -2387,10 +2428,10 @@ Fixpoint size_AnnExpr' {a}{b} (e: AnnExpr' a b) :=
           (Lists.List.map (fun p => size_AnnExpr' (snd (snd p))) pairs) +
            size_AnnExpr' body)
 
-(*  | AnnCast (_,e) _ => S (size_AnnExpr' e)
-  | AnnTick _ (_,e) => S (size_AnnExpr' e)
+  | AnnCast (_,e) _ => S (size_AnnExpr' e)
+(*  | AnnTick _ (_,e) => S (size_AnnExpr' e) *)
   | AnnType _ => 0
-  | AnnCoercion _ => 0 *)
+  | AnnCoercion _ => 0 
   end.
 
 (* ---------------------------------- *)
@@ -2946,6 +2987,8 @@ Axiom mkUnbranchedAxInstCo : Role ->
 
 Axiom mkTyVarTys : list TyVar -> list Type_.
 
+Axiom mkTyVarTy : TyVar -> Type_.
+
 Axiom mkTyConTy : TyCon -> Type_.
 
 Axiom mkTyConBindersPreferAnon : list TyVar -> Type_ -> list TyConBinder.
@@ -3478,6 +3521,16 @@ Definition visibleDataCons : AlgTyConRhs -> list DataCon :=
 Definition varUnique : Var -> Unique.Unique :=
   fun var => Unique.mkUniqueGrimily (realUnique var).
 
+Definition varToCoreExpr {b} : CoreBndr -> Expr b :=
+  fun v =>
+    if andb Util.debugIsOn (negb (true)) : bool
+    then (Panic.assertPanic (GHC.Base.hs_string__ "ghc/compiler/coreSyn/CoreSyn.hs")
+          #1920)
+    else Mk_Var v.
+
+Definition varsToCoreExprs {b} : list CoreBndr -> list (Expr b) :=
+  fun vs => GHC.Base.map varToCoreExpr vs.
+
 Definition vanillaCprProdRes : BasicTypes.Arity -> DmdResult :=
   fun _arity => Dunno RetProd.
 
@@ -3532,16 +3585,24 @@ Definition updateVarTypeM {m} `{GHC.Base.Monad m}
   fun f id =>
     f (varType id) GHC.Base.>>=
     (fun ty' =>
-       GHC.Base.return_ (let 'Mk_Id varName_0__ realUnique_1__ varType_2__ idScope_3__
-                            id_details_4__ id_info_5__ := id in
-                         Mk_Id varName_0__ realUnique_1__ ty' idScope_3__ id_details_4__ id_info_5__)).
+       GHC.Base.return_ (match id with
+                         | Mk_TyVar varName_0__ realUnique_1__ varType_2__ =>
+                             Mk_TyVar varName_0__ realUnique_1__ ty'
+                         | Mk_Id varName_3__ realUnique_4__ varType_5__ idScope_6__ id_details_7__
+                         id_info_8__ =>
+                             Mk_Id varName_3__ realUnique_4__ ty' idScope_6__ id_details_7__ id_info_8__
+                         end)).
 
 Definition updateVarType : (Type_ -> Type_) -> Id -> Id :=
   fun f id =>
-    let 'Mk_Id varName_0__ realUnique_1__ varType_2__ idScope_3__ id_details_4__
-       id_info_5__ := id in
-    Mk_Id varName_0__ realUnique_1__ (f (varType id)) idScope_3__ id_details_4__
-          id_info_5__.
+    match id with
+    | Mk_TyVar varName_0__ realUnique_1__ varType_2__ =>
+        Mk_TyVar varName_0__ realUnique_1__ (f (varType id))
+    | Mk_Id varName_3__ realUnique_4__ varType_5__ idScope_6__ id_details_7__
+    id_info_8__ =>
+        Mk_Id varName_3__ realUnique_4__ (f (varType id)) idScope_6__ id_details_7__
+              id_info_8__
+    end.
 
 Definition unwrapNewTyCon_maybe
    : TyCon -> option (list TyVar * Type_ * CoAxiom Unbranched)%type :=
@@ -3613,19 +3674,27 @@ Definition tyVarKind : TyVar -> Kind :=
 
 Definition updateTyVarKind : (Kind -> Kind) -> TyVar -> TyVar :=
   fun update tv =>
-    let 'Mk_Id varName_0__ realUnique_1__ varType_2__ idScope_3__ id_details_4__
-       id_info_5__ := tv in
-    Mk_Id varName_0__ realUnique_1__ (update (tyVarKind tv)) idScope_3__
-          id_details_4__ id_info_5__.
+    match tv with
+    | Mk_TyVar varName_0__ realUnique_1__ varType_2__ =>
+        Mk_TyVar varName_0__ realUnique_1__ (update (tyVarKind tv))
+    | Mk_Id varName_3__ realUnique_4__ varType_5__ idScope_6__ id_details_7__
+    id_info_8__ =>
+        Mk_Id varName_3__ realUnique_4__ (update (tyVarKind tv)) idScope_6__
+              id_details_7__ id_info_8__
+    end.
 
 Definition updateTyVarKindM {m} `{(GHC.Base.Monad m)}
    : (Kind -> m Kind) -> TyVar -> m TyVar :=
   fun update tv =>
     update (tyVarKind tv) GHC.Base.>>=
     (fun k' =>
-       GHC.Base.return_ (let 'Mk_Id varName_0__ realUnique_1__ varType_2__ idScope_3__
-                            id_details_4__ id_info_5__ := tv in
-                         Mk_Id varName_0__ realUnique_1__ k' idScope_3__ id_details_4__ id_info_5__)).
+       GHC.Base.return_ (match tv with
+                         | Mk_TyVar varName_0__ realUnique_1__ varType_2__ =>
+                             Mk_TyVar varName_0__ realUnique_1__ k'
+                         | Mk_Id varName_3__ realUnique_4__ varType_5__ idScope_6__ id_details_7__
+                         id_info_8__ =>
+                             Mk_Id varName_3__ realUnique_4__ k' idScope_6__ id_details_7__ id_info_8__
+                         end)).
 
 Definition tyConTuple_maybe : TyCon -> option BasicTypes.TupleSort :=
   fun arg_0__ =>
@@ -4079,23 +4148,36 @@ Definition sizeDVarSet : DVarSet -> nat :=
 
 Definition setVarUnique : Var -> Unique.Unique -> Var :=
   fun var uniq =>
-    let 'Mk_Id varName_0__ realUnique_1__ varType_2__ idScope_3__ id_details_4__
-       id_info_5__ := var in
-    Mk_Id (Name.setNameUnique (varName var) uniq) (Unique.getKey uniq) varType_2__
-          idScope_3__ id_details_4__ id_info_5__.
+    match var with
+    | Mk_TyVar varName_0__ realUnique_1__ varType_2__ =>
+        Mk_TyVar (Name.setNameUnique (varName var) uniq) (Unique.getKey uniq)
+                 varType_2__
+    | Mk_Id varName_3__ realUnique_4__ varType_5__ idScope_6__ id_details_7__
+    id_info_8__ =>
+        Mk_Id (Name.setNameUnique (varName var) uniq) (Unique.getKey uniq) varType_5__
+              idScope_6__ id_details_7__ id_info_8__
+    end.
 
 Definition setVarType : Id -> Type_ -> Id :=
   fun id ty =>
-    let 'Mk_Id varName_0__ realUnique_1__ varType_2__ idScope_3__ id_details_4__
-       id_info_5__ := id in
-    Mk_Id varName_0__ realUnique_1__ ty idScope_3__ id_details_4__ id_info_5__.
+    match id with
+    | Mk_TyVar varName_0__ realUnique_1__ varType_2__ =>
+        Mk_TyVar varName_0__ realUnique_1__ ty
+    | Mk_Id varName_3__ realUnique_4__ varType_5__ idScope_6__ id_details_7__
+    id_info_8__ =>
+        Mk_Id varName_3__ realUnique_4__ ty idScope_6__ id_details_7__ id_info_8__
+    end.
 
 Definition setVarName : Var -> Name.Name -> Var :=
   fun var new_name =>
-    let 'Mk_Id varName_0__ realUnique_1__ varType_2__ idScope_3__ id_details_4__
-       id_info_5__ := var in
-    Mk_Id new_name (Unique.getKey (Unique.getUnique new_name)) varType_2__
-          idScope_3__ id_details_4__ id_info_5__.
+    match var with
+    | Mk_TyVar varName_0__ realUnique_1__ varType_2__ =>
+        Mk_TyVar new_name (Unique.getKey (Unique.getUnique new_name)) varType_2__
+    | Mk_Id varName_3__ realUnique_4__ varType_5__ idScope_6__ id_details_7__
+    id_info_8__ =>
+        Mk_Id new_name (Unique.getKey (Unique.getUnique new_name)) varType_5__
+              idScope_6__ id_details_7__ id_info_8__
+    end.
 
 Definition setUnfoldingInfo : IdInfo -> Unfolding -> IdInfo :=
   fun info uf =>
@@ -4114,9 +4196,13 @@ Definition setTyVarName : TyVar -> Name.Name -> TyVar :=
 
 Definition setTyVarKind : TyVar -> Kind -> TyVar :=
   fun tv k =>
-    let 'Mk_Id varName_0__ realUnique_1__ varType_2__ idScope_3__ id_details_4__
-       id_info_5__ := tv in
-    Mk_Id varName_0__ realUnique_1__ k idScope_3__ id_details_4__ id_info_5__.
+    match tv with
+    | Mk_TyVar varName_0__ realUnique_1__ varType_2__ =>
+        Mk_TyVar varName_0__ realUnique_1__ k
+    | Mk_Id varName_3__ realUnique_4__ varType_5__ idScope_6__ id_details_7__
+    id_info_8__ =>
+        Mk_Id varName_3__ realUnique_4__ k idScope_6__ id_details_7__ id_info_8__
+    end.
 
 Definition setStrictnessInfo : IdInfo -> StrictSig -> IdInfo :=
   fun info dd =>
@@ -4213,18 +4299,25 @@ Definition setIdExported : Id -> Id :=
   fun arg_0__ =>
     match arg_0__ with
     | (Mk_Id _ _ _ (LocalId _) _ _ as id) =>
-        let 'Mk_Id varName_1__ realUnique_2__ varType_3__ idScope_4__ id_details_5__
-           id_info_6__ := id in
-        Mk_Id varName_1__ realUnique_2__ varType_3__ (LocalId Exported) id_details_5__
-              id_info_6__
+        match id with
+        | Mk_TyVar _ _ _ => GHC.Err.error (GHC.Base.hs_string__ "Partial record update")
+        | Mk_Id varName_1__ realUnique_2__ varType_3__ idScope_4__ id_details_5__
+        id_info_6__ =>
+            Mk_Id varName_1__ realUnique_2__ varType_3__ (LocalId Exported) id_details_5__
+                  id_info_6__
+        end
     | (Mk_Id _ _ _ GlobalId _ _ as id) => id
+    | tv => Panic.panicStr (GHC.Base.hs_string__ "setIdExported") (Panic.someSDoc)
     end.
 
 Definition setIdDetails : Id -> IdDetails -> Id :=
   fun id details =>
-    let 'Mk_Id varName_0__ realUnique_1__ varType_2__ idScope_3__ id_details_4__
-       id_info_5__ := id in
-    Mk_Id varName_0__ realUnique_1__ varType_2__ idScope_3__ details id_info_5__.
+    match id with
+    | Mk_TyVar _ _ _ => GHC.Err.error (GHC.Base.hs_string__ "Partial record update")
+    | Mk_Id varName_0__ realUnique_1__ varType_2__ idScope_3__ id_details_4__
+    id_info_5__ =>
+        Mk_Id varName_0__ realUnique_1__ varType_2__ idScope_3__ details id_info_5__
+    end.
 
 Definition setDemandInfo : IdInfo -> Demand -> IdInfo :=
   fun info dd =>
@@ -4687,6 +4780,9 @@ Definition zipVarEnv {a} : list Var -> list a -> VarEnv a :=
   fun tyvars tys =>
     mkVarEnv (Util.zipEqual (GHC.Base.hs_string__ "zipVarEnv") tyvars tys).
 
+Definition mkVarApps {b} : Expr b -> list Var -> Expr b :=
+  fun f vars => Data.Foldable.foldl (fun e a => App e (varToCoreExpr a)) f vars.
+
 Local Definition Eq___Count_op_zeze__ : Count -> Count -> bool :=
   fun arg_0__ arg_1__ =>
     match arg_0__, arg_1__ with
@@ -4761,7 +4857,42 @@ Program Definition mkWorkerDemand : nat -> Demand :=
             JD Lazy (Mk_Use One (go n)).
 Solve Obligations with (solve_mkWorkerDemand).
 
+Definition mkTyVarBinder : ArgFlag -> Var -> TyVarBinder :=
+  fun vis var => TvBndr var vis.
+
+Definition mkTyVarBinders : ArgFlag -> list TyVar -> list TyVarBinder :=
+  fun vis => GHC.Base.map (mkTyVarBinder vis).
+
+Definition tyConTyVarBinders : list TyConBinder -> list TyVarBinder :=
+  fun tc_bndrs =>
+    let mk_binder :=
+      fun '(TvBndr tv tc_vis) =>
+        let vis :=
+          match tc_vis with
+          | AnonTCB => Specified
+          | NamedTCB Required => Specified
+          | NamedTCB vis => vis
+          end in
+        mkTyVarBinder vis tv in
+    GHC.Base.map mk_binder tc_bndrs.
+
+Definition mkTyVar : Name.Name -> Kind -> TyVar :=
+  fun name kind => Mk_TyVar name (Unique.getKey (Name.nameUnique name)) kind.
+
 Axiom mkTyConKind : list TyConBinder -> Kind -> Kind.
+
+Definition mkTyBind : TyVar -> Type_ -> CoreBind :=
+  fun tv ty => NonRec tv (Mk_Type ty).
+
+Definition mkTyArg {b} : Type_ -> Expr b :=
+  fun ty =>
+    match isCoercionTy_maybe ty with
+    | Some co => Mk_Coercion co
+    | _ => Mk_Type ty
+    end.
+
+Definition mkTyApps {b} : Expr b -> list Type_ -> Expr b :=
+  fun f args => Data.Foldable.foldl (fun e a => App e (mkTyArg a)) f args.
 
 Definition mkSumTyCon
    : Name.Name ->
@@ -4962,6 +5093,12 @@ Definition mkDoubleLit {b} : GHC.Real.Rational -> Expr b :=
 
 Definition mkDmdType : DmdEnv -> list Demand -> DmdResult -> DmdType :=
   fun fv ds res => Mk_DmdType fv ds res.
+
+Definition mkCoBind : CoVar -> Coercion -> CoreBind :=
+  fun cv co => NonRec cv (Mk_Coercion co).
+
+Definition mkCoApps {b} : Expr b -> list Coercion -> Expr b :=
+  fun f args => Data.Foldable.foldl (fun e a => App e (Mk_Coercion a)) f args.
 
 Definition mkClass
    : Name.Name ->
@@ -5192,9 +5329,12 @@ Definition lookupRnInScope : RnEnv2 -> Var -> Var :=
 
 Definition lazySetIdInfo : Id -> IdInfo -> Var :=
   fun id info =>
-    let 'Mk_Id varName_0__ realUnique_1__ varType_2__ idScope_3__ id_details_4__
-       id_info_5__ := id in
-    Mk_Id varName_0__ realUnique_1__ varType_2__ idScope_3__ id_details_4__ info.
+    match id with
+    | Mk_TyVar _ _ _ => GHC.Err.error (GHC.Base.hs_string__ "Partial record update")
+    | Mk_Id varName_0__ realUnique_1__ varType_2__ idScope_3__ id_details_4__
+    id_info_5__ =>
+        Mk_Id varName_0__ realUnique_1__ varType_2__ idScope_3__ id_details_4__ info
+    end.
 
 Definition lazyApply2Dmd : Demand :=
   JD Lazy (Mk_Use One (UCall One (UCall One Used))).
@@ -5389,7 +5529,7 @@ Definition isTypeSynonymTyCon : TyCon -> bool :=
     end.
 
 Definition isTypeArg {b} : Expr b -> bool :=
-  fun arg_0__ => false.
+  fun arg_0__ => match arg_0__ with | Mk_Type _ => true | _ => false end.
 
 Definition isValArg {b} : Expr b -> bool :=
   fun e => negb (isTypeArg e).
@@ -5398,13 +5538,18 @@ Definition valArgCount {b} : list (Arg b) -> nat :=
   Util.count isValArg.
 
 Definition isTyVar : Var -> bool :=
-  fun arg_0__ => false.
+  fun arg_0__ => match arg_0__ with | Mk_TyVar _ _ _ => true | _ => false end.
 
 Definition isTyConAssoc : TyCon -> bool :=
   fun tc => Data.Maybe.isJust (tyConAssoc_maybe tc).
 
 Definition isTyCoArg {b} : Expr b -> bool :=
-  fun arg_0__ => false.
+  fun arg_0__ =>
+    match arg_0__ with
+    | Mk_Type _ => true
+    | Mk_Coercion _ => true
+    | _ => false
+    end.
 
 Definition isTupleTyCon : TyCon -> bool :=
   fun arg_0__ =>
@@ -5644,10 +5789,13 @@ Definition setIdNotExported : Id -> Id :=
     if andb Util.debugIsOn (negb (isLocalId id)) : bool
     then (Panic.assertPanic (GHC.Base.hs_string__ "ghc/compiler/basicTypes/Var.hs")
           #591)
-    else let 'Mk_Id varName_0__ realUnique_1__ varType_2__ idScope_3__
-            id_details_4__ id_info_5__ := id in
-         Mk_Id varName_0__ realUnique_1__ varType_2__ (LocalId NotExported)
-               id_details_4__ id_info_5__.
+    else match id with
+         | Mk_TyVar _ _ _ => GHC.Err.error (GHC.Base.hs_string__ "Partial record update")
+         | Mk_Id varName_0__ realUnique_1__ varType_2__ idScope_3__ id_details_4__
+         id_info_5__ =>
+             Mk_Id varName_0__ realUnique_1__ varType_2__ (LocalId NotExported)
+                   id_details_4__ id_info_5__
+         end.
 
 Definition isLazy : ArgStr -> bool :=
   fun arg_0__ => match arg_0__ with | Lazy => true | Mk_Str _ _ => false end.
@@ -5689,26 +5837,13 @@ Definition isImplicitTyCon : TyCon -> bool :=
     end.
 
 Definition isId : Var -> bool :=
-  fun '(Mk_Id _ _ _ _ _ _) => true.
+  fun arg_0__ => match arg_0__ with | Mk_Id _ _ _ _ _ _ => true | _ => false end.
 
 Definition isRuntimeVar : Var -> bool :=
   isId.
 
 Definition valBndrCount : list CoreBndr -> nat :=
   Util.count isId.
-
-Definition varToCoreExpr {b} : CoreBndr -> Expr b :=
-  fun v =>
-    if andb Util.debugIsOn (negb (isId v)) : bool
-    then (Panic.assertPanic (GHC.Base.hs_string__ "ghc/compiler/coreSyn/CoreSyn.hs")
-          #1920)
-    else Mk_Var v.
-
-Definition mkVarApps {b} : Expr b -> list Var -> Expr b :=
-  fun f vars => Data.Foldable.foldl (fun e a => App e (varToCoreExpr a)) f vars.
-
-Definition varsToCoreExprs {b} : list CoreBndr -> list (Expr b) :=
-  fun vs => GHC.Base.map varToCoreExpr vs.
 
 Definition isHyperStr : ArgStr -> bool :=
   fun arg_0__ => match arg_0__ with | Mk_Str _ HyperStr => true | _ => false end.
@@ -5957,13 +6092,21 @@ Definition isCompulsoryUnfolding : Unfolding -> bool :=
   fun arg_0__ => false.
 
 Definition isCoVarDetails : IdDetails -> bool :=
-  fun arg_0__ => false.
+  fun arg_0__ => match arg_0__ with | CoVarId => true | _ => false end.
 
 Definition isNonCoVarId : Var -> bool :=
-  fun '(Mk_Id _ _ _ _ details _) => negb (isCoVarDetails details).
+  fun arg_0__ =>
+    match arg_0__ with
+    | Mk_Id _ _ _ _ details _ => negb (isCoVarDetails details)
+    | _ => false
+    end.
 
 Definition isCoVar : Var -> bool :=
-  fun '(Mk_Id _ _ _ _ details _) => isCoVarDetails details.
+  fun arg_0__ =>
+    match arg_0__ with
+    | Mk_Id _ _ _ _ details _ => isCoVarDetails details
+    | _ => false
+    end.
 
 Definition isTyCoVar : Var -> bool :=
   fun v => orb (isTyVar v) (isCoVar v).
@@ -6097,10 +6240,18 @@ Definition increaseStrictSigArity : nat -> StrictSig -> StrictSig :=
     end.
 
 Definition idInfo `{Util.HasDebugCallStack} : Id -> IdInfo :=
-  fun '(Mk_Id _ _ _ _ _ info) => info.
+  fun arg_0__ =>
+    match arg_0__ with
+    | Mk_Id _ _ _ _ _ info => info
+    | other => Panic.panicStr (GHC.Base.hs_string__ "idInfo") (Panic.someSDoc)
+    end.
 
 Definition idDetails : Id -> IdDetails :=
-  fun '(Mk_Id _ _ _ _ details _) => details.
+  fun arg_0__ =>
+    match arg_0__ with
+    | Mk_Id _ _ _ _ details _ => details
+    | other => Panic.panicStr (GHC.Base.hs_string__ "idDetails") (Panic.someSDoc)
+    end.
 
 Definition hasSomeUnfolding : Unfolding -> bool :=
   fun '(NoUnfolding) => false.
@@ -6109,10 +6260,13 @@ Definition hasDemandEnvSig : StrictSig -> bool :=
   fun '(Mk_StrictSig (Mk_DmdType env _ _)) => negb (isEmptyVarEnv env).
 
 Definition globaliseId : Id -> Id :=
-  fun '(Mk_Id varName_0__ realUnique_1__ varType_2__ idScope_3__ id_details_4__
-  id_info_5__) =>
-    Mk_Id varName_0__ realUnique_1__ varType_2__ GlobalId id_details_4__
-          id_info_5__.
+  fun id =>
+    match id with
+    | Mk_TyVar _ _ _ => GHC.Err.error (GHC.Base.hs_string__ "Partial record update")
+    | Mk_Id varName_0__ realUnique_1__ varType_2__ idScope_3__ id_details_4__
+    id_info_5__ =>
+        Mk_Id varName_0__ realUnique_1__ varType_2__ GlobalId id_details_4__ id_info_5__
+    end.
 
 Definition getUseDmd {s} {u} : JointDmd s u -> u :=
   ud.
@@ -6250,7 +6404,7 @@ Definition modifyDVarEnv {a} : (a -> a) -> DVarEnv a -> Var -> DVarEnv a :=
     end.
 
 Definition exprToCoercion_maybe : CoreExpr -> option Coercion :=
-  fun arg_0__ => None.
+  fun arg_0__ => match arg_0__ with | Mk_Coercion co => Some co | _ => None end.
 
 Definition expandUnfolding_maybe : Unfolding -> option CoreExpr :=
   fun arg_0__ => None.
@@ -6757,11 +6911,14 @@ Definition deTagExpr {t} : TaggedExpr t -> CoreExpr :=
            match arg_0__ with
            | Mk_Var v => Mk_Var v
            | Lit l => Lit l
+           | Mk_Type ty => Mk_Type ty
+           | Mk_Coercion co => Mk_Coercion co
            | App e1 e2 => App (deTagExpr e1) (deTagExpr e2)
            | Lam (TB b _) e => Lam b (deTagExpr e)
            | Let bind body => Let (deTagBind bind) (deTagExpr body)
            | Case e (TB b _) ty alts =>
                Case (deTagExpr e) b ty (GHC.Base.map deTagAlt alts)
+           | Cast e co => Cast (deTagExpr e) co
            end.
 
 Definition deTagBind {t} : TaggedBind t -> CoreBind :=
@@ -6790,10 +6947,13 @@ Definition deAnnotate'
              let 'pair (pair con args) rhs := arg_0__ in
              pair (pair con args) (deAnnotate rhs) in
            match arg_0__ with
+           | AnnType t => Mk_Type t
+           | AnnCoercion co => Mk_Coercion co
            | AnnVar v => Mk_Var v
            | AnnLit lit => Lit lit
            | AnnLam binder body => Lam binder (deAnnotate body)
            | AnnApp fun_ arg => App (deAnnotate fun_) (deAnnotate arg)
+           | AnnCast e (pair _ co) => Cast (deAnnotate e) co
            | AnnLet bind body => Let (deAnnBind bind) (deAnnotate body)
            | AnnCase scrut v t alts =>
                Case (deAnnotate scrut) v t (GHC.Base.map deAnnAlt alts)
@@ -6822,10 +6982,13 @@ Definition deAnnBind : forall {b} {annot}, AnnBind b annot -> Bind b :=
              let 'pair (pair con args) rhs := arg_0__ in
              pair (pair con args) (deAnnotate rhs) in
            match arg_0__ with
+           | AnnType t => Mk_Type t
+           | AnnCoercion co => Mk_Coercion co
            | AnnVar v => Mk_Var v
            | AnnLit lit => Lit lit
            | AnnLam binder body => Lam binder (deAnnotate body)
            | AnnApp fun_ arg => App (deAnnotate fun_) (deAnnotate arg)
+           | AnnCast e (pair _ co) => Cast (deAnnotate e) co
            | AnnLet bind body => Let (deAnnBind bind) (deAnnotate body)
            | AnnCase scrut v t alts =>
                Case (deAnnotate scrut) v t (GHC.Base.map deAnnAlt alts)
@@ -6867,7 +7030,7 @@ Definition mkConApp {b} : DataCon -> list (Arg b) -> Expr b :=
 
 Definition mkConApp2 {b} : DataCon -> list Type_ -> list Var -> Expr b :=
   fun con tys arg_ids =>
-    mkApps (mkApps (Mk_Var (dataConWorkId con)) (GHC.Base.map GHC.Err.default tys))
+    mkApps (mkApps (Mk_Var (dataConWorkId con)) (GHC.Base.map Mk_Type tys))
            (GHC.Base.map varToCoreExpr arg_ids).
 
 Definition dataConUserTyVarBinders : DataCon -> list TyVarBinder :=
@@ -7100,6 +7263,12 @@ Program Definition collectAnnArgs {b} {a}
                                end) in
             go expr nil.
 Solve Obligations with (solve_collectAnnArgsTicks).
+
+Definition coVarDetails : IdDetails :=
+  CoVarId.
+
+Definition mkCoVar : Name.Name -> Type_ -> CoVar :=
+  fun name ty => mk_id name ty (LocalId NotExported) coVarDetails vanillaIdInfo.
 
 Definition cmpAltCon : AltCon -> AltCon -> comparison :=
   fun arg_0__ arg_1__ =>
