examples/ghc/lib/CoreStats.v
@@ -109,6 +109,9 @@ Definition exprSize : CoreExpr -> nat :=
            | Lam b e => bndrSize b + exprSize e
            | Let b e => bindSize b + exprSize e
            | Case e b _ as_ => exprSize e + bndrSize b + 1 + sum (map altSize as_)
+           | Cast e _ => 1 + exprSize e
+           | Mk_Type _ => 1
+           | Mk_Coercion _ => 1
            end with bindSize (arg_0__ : CoreBind) : nat
                       := let pairSize (arg_0__ : (Var * CoreExpr)%type) : nat :=
                            let 'pair b e := arg_0__ in
@@ -133,6 +136,9 @@ Definition bindSize : CoreBind -> nat :=
            | Lam b e => bndrSize b + exprSize e
            | Let b e => bindSize b + exprSize e
            | Case e b _ as_ => exprSize e + bndrSize b + 1 + sum (map altSize as_)
+           | Cast e _ => 1 + exprSize e
+           | Mk_Type _ => 1
+           | Mk_Coercion _ => 1
            end with bindSize (arg_0__ : CoreBind) : nat
                       := let pairSize (arg_0__ : (Var * CoreExpr)%type) : nat :=
                            let 'pair b e := arg_0__ in
@@ -159,11 +165,14 @@ Definition bindStats : BasicTypes.TopLevelFlag -> CoreBind -> CoreStats :=
            match arg_0__ with
            | Mk_Var _ => oneTM
            | Lit _ => oneTM
+           | Mk_Type t => tyStats t
+           | Mk_Coercion c => coStats c
            | App f a => plusCS (exprStats f) (exprStats a)
            | Lam b e => plusCS (bndrStats b) (exprStats e)
            | Let b e => plusCS (bindStats BasicTypes.NotTopLevel b) (exprStats e)
            | Case e b _ as_ =>
                plusCS (plusCS (exprStats e) (bndrStats b)) (sumCS altStats as_)
+           | Cast e co => plusCS (coStats co) (exprStats e)
            end with bindStats (arg_0__ : BasicTypes.TopLevelFlag) (arg_1__ : CoreBind)
                       : CoreStats
                       := let bindingStats (top_lvl : BasicTypes.TopLevelFlag) (v : Var) (r : CoreExpr)
@@ -185,11 +194,14 @@ Definition exprStats : CoreExpr -> CoreStats :=
            match arg_0__ with
            | Mk_Var _ => oneTM
            | Lit _ => oneTM
+           | Mk_Type t => tyStats t
+           | Mk_Coercion c => coStats c
            | App f a => plusCS (exprStats f) (exprStats a)
            | Lam b e => plusCS (bndrStats b) (exprStats e)
            | Let b e => plusCS (bindStats BasicTypes.NotTopLevel b) (exprStats e)
            | Case e b _ as_ =>
                plusCS (plusCS (exprStats e) (bndrStats b)) (sumCS altStats as_)
+           | Cast e co => plusCS (coStats co) (exprStats e)
            end with bindStats (arg_0__ : BasicTypes.TopLevelFlag) (arg_1__ : CoreBind)
                       : CoreStats
                       := let bindingStats (top_lvl : BasicTypes.TopLevelFlag) (v : Var) (r : CoreExpr)
@@ -211,10 +223,10 @@ Definition bindingStats
    `CoreStats.Outputable__CoreStats' *)
 
 (* External variables:
-     App Case CoreAlt CoreBind CoreExpr Id Lam Let Lit Mk_Var NonRec ProfNote Rec
-     Tickish Var bool foldl' isTyVar list map nat op_z2218U__ op_zp__ op_zt__ orb
-     pair sum varType AxiomatizedTypes.Coercion AxiomatizedTypes.Type_
-     BasicTypes.NotTopLevel BasicTypes.TopLevel BasicTypes.TopLevelFlag
-     BasicTypes.isTopLevel GHC.Err.Build_Default GHC.Err.Default GHC.Err.default
-     Id.isJoinId
+     App Case Cast CoreAlt CoreBind CoreExpr Id Lam Let Lit Mk_Coercion Mk_Type
+     Mk_Var NonRec ProfNote Rec Tickish Var bool foldl' isTyVar list map nat
+     op_z2218U__ op_zp__ op_zt__ orb pair sum varType AxiomatizedTypes.Coercion
+     AxiomatizedTypes.Type_ BasicTypes.NotTopLevel BasicTypes.TopLevel
+     BasicTypes.TopLevelFlag BasicTypes.isTopLevel GHC.Err.Build_Default
+     GHC.Err.Default GHC.Err.default Id.isJoinId
 *)
