examples/ghc/manual/CallArity.v
@@ -181,12 +181,15 @@ Definition callArityAnal
      Core.VarSet -> Core.CoreExpr -> (CallArityRes * Core.CoreExpr)%type :=
   fix callArityAnal (arg_0__ : BasicTypes.Arity) (arg_1__ : Core.VarSet) (arg_2__
                       : Core.CoreExpr) : (CallArityRes * Core.CoreExpr)%type
-        := let j_24__ :=
+        := let j_26__ :=
              match arg_0__, arg_1__, arg_2__ with
              | arity, int, Core.Lam v e =>
                  let 'pair ae e' := callArityAnal (arity GHC.Num.- #1) (Core.delVarSet int v)
                                       e in
                  pair ae (Core.Lam v e')
+             | arity, int, Core.App e (Core.Mk_Type t) =>
+                 Control.Arrow.arrow_second (fun e => Core.App e (Core.Mk_Type t)) (callArityAnal
+                                                                                    arity int e)
              | arity, int, Core.App e1 e2 =>
                  let 'pair ae2 e2' := callArityAnal #0 int e2 in
                  let ae2' :=
@@ -212,17 +215,21 @@ Definition callArityAnal
                  pair final_ae (Core.Let bind' e')
              | _, _, _ => GHC.Err.patternFailure
              end in
-           let j_28__ :=
+           let j_30__ :=
              match arg_0__, arg_1__, arg_2__ with
              | num_3__, int, Core.Lam v e =>
                  let 'pair ae e' := callArityAnal #0 (Core.delVarSet int v) e in
                  let ae' := calledMultipleTimes ae in
                  if num_3__ GHC.Base.== #0 : bool then pair ae' (Core.Lam v e') else
-                 j_24__
-             | _, _, _ => j_24__
+                 j_26__
+             | _, _, _ => j_26__
              end in
            match arg_0__, arg_1__, arg_2__ with
            | _, _, (Core.Lit _ as e) => pair emptyArityRes e
+           | _, _, (Core.Mk_Type _ as e) => pair emptyArityRes e
+           | _, _, (Core.Mk_Coercion _ as e) => pair emptyArityRes e
+           | arity, int, Core.Cast e co =>
+               Control.Arrow.arrow_second (fun e => Core.Cast e co) (callArityAnal arity int e)
            | arity, int, (Core.Mk_Var v as e) =>
                if Core.elemVarSet v int : bool then pair (unitArityRes v arity) e else
                pair emptyArityRes e
@@ -230,8 +237,8 @@ Definition callArityAnal
                if negb (Core.isId v) : bool
                then Control.Arrow.arrow_second (Core.Lam v) (callArityAnal arity
                                                                            (Core.delVarSet int v) e) else
-               j_28__
-           | _, _, _ => j_28__
+               j_30__
+           | _, _, _ => j_30__
            end.
 
 Definition callArityRHS : Core.CoreExpr -> Core.CoreExpr :=
@@ -364,16 +371,17 @@ Definition callArityAnalProgram
      None Some andb bool callArityBind1 cons false list negb nil op_zt__ option pair
      true BasicTypes.Arity Control.Arrow.arrow_first Control.Arrow.arrow_second
      Coq.Init.Datatypes.app Coq.Lists.List.flat_map Coq.Lists.List.length Core.App
-     Core.Case Core.CoreBind Core.CoreExpr Core.CoreProgram Core.Id Core.Lam Core.Let
-     Core.Lit Core.Mk_Var Core.NonRec Core.Rec Core.Var Core.VarEnv Core.VarSet
-     Core.bindersOf Core.delVarEnv Core.delVarSet Core.delVarSetList Core.elemVarSet
-     Core.emptyVarEnv Core.emptyVarSet Core.extendVarSetList Core.isBotRes
-     Core.isExportedId Core.isId Core.lookupVarEnv Core.mkVarEnv Core.mkVarSet
-     Core.plusVarEnv_C Core.splitStrictSig Core.unitVarEnv CoreArity.typeArity
-     CoreUtils.exprIsCheap CoreUtils.exprIsTrivial Data.Foldable.any
-     Data.Foldable.foldl Data.Foldable.foldr Data.Foldable.null Data.Foldable.or
-     Data.Tuple.fst Data.Tuple.snd DynFlags.DynFlags GHC.Base.const GHC.Base.map
-     GHC.Base.min GHC.Base.op_z2218U__ GHC.Base.op_zeze__ GHC.Base.op_zsze__
+     Core.Case Core.Cast Core.CoreBind Core.CoreExpr Core.CoreProgram Core.Id
+     Core.Lam Core.Let Core.Lit Core.Mk_Coercion Core.Mk_Type Core.Mk_Var Core.NonRec
+     Core.Rec Core.Var Core.VarEnv Core.VarSet Core.bindersOf Core.delVarEnv
+     Core.delVarSet Core.delVarSetList Core.elemVarSet Core.emptyVarEnv
+     Core.emptyVarSet Core.extendVarSetList Core.isBotRes Core.isExportedId Core.isId
+     Core.lookupVarEnv Core.mkVarEnv Core.mkVarSet Core.plusVarEnv_C
+     Core.splitStrictSig Core.unitVarEnv CoreArity.typeArity CoreUtils.exprIsCheap
+     CoreUtils.exprIsTrivial Data.Foldable.any Data.Foldable.foldl
+     Data.Foldable.foldr Data.Foldable.null Data.Foldable.or Data.Tuple.fst
+     Data.Tuple.snd DynFlags.DynFlags GHC.Base.const GHC.Base.map GHC.Base.min
+     GHC.Base.op_z2218U__ GHC.Base.op_zeze__ GHC.Base.op_zsze__
      GHC.DeferredFix.deferredFix1 GHC.Err.patternFailure GHC.List.filter
      GHC.List.unzip GHC.Num.fromInteger GHC.Num.op_zm__ GHC.Num.op_zp__
      Id.idCallArity Id.idStrictness Id.idType Id.setIdCallArity UnVarGraph.UnVarGraph
