examples/ghc/manual/NestedRecursionHelpers.v
@@ -138,7 +138,8 @@ Proof.
     [ v | lit
     | e1 IH1 e2 IH2 | v e IH
     | bind body IH | scrut IHscrut bndr t alts
-     ]
+    | e IH a (* | tickish e IH *)
+    | a | a ]
     [| n]
     bs;
     try by [right; split; econstructor | left].
