examples/ghc/theories/CoreInduct.v
@@ -29,7 +29,11 @@ Lemma core_induct' {b} :
        end) ->
       P body ->
       P (Let binds body))
-  (HCase : forall scrut bndr ty alts, P scrut -> (forall dc pats rhs, In (dc, pats ,rhs) alts -> P rhs) -> P (Case scrut bndr ty alts)),
+  (HCase : forall scrut bndr ty alts, P scrut -> (forall dc pats rhs, In (dc, pats ,rhs) alts -> P rhs) -> P (Case scrut bndr ty alts))
+  (HCast : forall e co, P e -> P (Cast e co))
+(*   (HTick : forall tickish e, P e -> P (Tick tickish e)) *)
+  (HType : forall ty, P (Mk_Type ty))
+  (HCoercion : forall co, P (Mk_Coercion co)),
   P e.
 Proof.
   intros.
@@ -62,6 +66,10 @@ Proof.
             rewrite <- H2.
             apply IH.
          ++ eapply IHalts'. eassumption.
+  * apply HCast; apply IH.
+(*   * apply HTick; apply IH. *)
+  * apply HType.
+  * apply HCoercion.
 Qed.
 
 Lemma core_induct :
@@ -78,7 +86,11 @@ Lemma core_induct :
        end) ->
       P body ->
       P (Let binds body))
-  (HCase : forall scrut bndr ty alts, P scrut -> (forall dc pats rhs, In (dc, pats ,rhs) alts -> P rhs) -> P (Case scrut bndr ty alts)),
+  (HCase : forall scrut bndr ty alts, P scrut -> (forall dc pats rhs, In (dc, pats ,rhs) alts -> P rhs) -> P (Case scrut bndr ty alts))
+  (HCast : forall e co, P e -> P (Cast e co)) 
+(*  (HTick : forall tickish e, P e -> P (Tick tickish e)) *)
+  (HType : forall ty, P (Mk_Type ty))
+  (HCoercion : forall co, P (Mk_Coercion co)),
   P e.
 Proof. exact core_induct'. Qed.
 
@@ -99,9 +111,12 @@ Section CoreLT.
     | Case scrut bndr ty alts  => 
         S (core_size scrut +
            fold_right plus 0 (map (fun p => core_size (snd p)) alts))
+    | Cast e _ =>   S (core_size e)
+(*    | Tick _ e =>   S (core_size e) *)
+    | Mk_Type _  =>   0
+    | Mk_Coercion _ => 0
     end.
-    
-  
+
   (* We use the size only for comparisons. So lets
      make a definition here that we never unfold otherwise,
      and isntead create a tactic that handles all cases.
