examples/ghc/theories/JoinPointInvariants.v
@@ -298,10 +298,10 @@ Fixpoint isJoinPointsValid (e : CoreExpr) (n : nat) (jps : VarSet) {struct e} : 
       let jps'' := delVarSetList jps' pats  in
       forallb (fun v => negb (isJoinId v)) pats &&
       isJoinPointsValid rhs 0 jps'') alts  (* Tail-call position *)
-(*  | Cast e _ =>    isJoinPointsValid e 0 jps
-  | Tick _ e =>    isJoinPointsValid e 0 jps
-  | Type_ _  =>   true
-  | Coercion _ => true *)
+  | Cast e _ =>    isJoinPointsValid e 0 jps
+(*  | Tick _ e =>    isJoinPointsValid e 0 jps *)
+  | Mk_Type _  =>   true
+  | Mk_Coercion _ => true 
   end
 with isJoinRHS_aux (a : JoinArity) (rhs : CoreExpr) (jps : VarSet) {struct rhs} : bool :=
   if a <? 1 then false else
@@ -555,11 +555,11 @@ Proof.
       assumption.
     - unfold varToCoreExpr.
       repeat destruct_match; try reflexivity.
-      + (* new case from debugIsOn *) destruct x; simpl in *;
+      + (* new case from debugIsOn *)
           try rewrite andb_false_r in Heq;
           try discriminate.
       + simpl. rewrite isJoinId_eq in H.
-      destruct_match; congruence.
+      destruct_match; congruence. 
 Qed.
 
 Lemma isJoinPointsValid_MkLetRec: forall pairs body jps,
@@ -807,18 +807,18 @@ Proof.
       epose proof (mapUnionVarSet_In_subVarSet f HIn) as H ; simpl in H end.
     rewrite delVarSetList_rev, <- delVarSetList_single, <- delVarSetList_app.
     set_b_iff; fsetdec.
-(*  - apply H. 
+  - apply H. 
     eapply disjointVarSet_subVarSet_l; only 1: apply H0.
     apply subVarSet_delVarSetList_both.
     rewrite exprFreeVars_Cast.
     set_b_iff; fsetdec.
-  - apply H. 
+(*  - apply H. 
     eapply disjointVarSet_subVarSet_l; only 1: apply H0.
     apply subVarSet_delVarSetList_both.
     rewrite exprFreeVars_Tick.
-    set_b_iff; fsetdec.
+    set_b_iff; fsetdec. *)
   - reflexivity.
-  - reflexivity. *)
+  - reflexivity. 
 Qed.
 
 Lemma isJoinPointsValid_fresh_updJPSs:
@@ -1018,10 +1018,10 @@ Proof.
      apply Respects_StrongSubset_delVarSetList with
           (P := fun jps => isJoinPointsValid rhs 0 jps = true).
      apply H0.
-(*   * apply H.
    * apply H.
+(*   * apply H. *)
    * apply Respects_StrongSubset_const.
-   * apply Respects_StrongSubset_const. *)
+   * apply Respects_StrongSubset_const. 
 Qed.
 
 Instance Respects_StrongSubset_isJoinPointsValid e n :
